AbsDen/IGDTT.lean
@@ -35,14 +35,15 @@ syntax (name := nextElem) ident Term.optType ppSpace Term.leftArrow term : nextE
 syntax (name := delayedSubst) "next[" nextElem,* "]." term : term
 macro_rules
   | `(term| next[]. $e) => `(Later.next (fun () => $e))
-  | `(term| next[ $x:ident ← $e₁ ]. $e₂) => `(pure (fun $x => $e₂) <*> $e₁)
-  | `(term| next[ $x:ident : $t ← $e₁ ]. $e₂) => `(pure (fun $x : $t => $e₂) <*> $e₁)
-  | `(term| next[ $x:ident ← $e₁, $es,* ]. $e₂) => `((next[ $es,* ]. (fun $x => $e₂)) <*> $e₁)
-  | `(term| next[ $x:ident : $t ← $e₁, $es,* ]. $e₂) => `((next[ $es,* ]. (fun $x : $t => $e₂)) <*> $e₁)
+  | `(term| next[ $x:ident ← $e₁ ]. $e₂) => `(Later.ap (next[]. (fun $x => $e₂)) $e₁)
+  | `(term| next[ $x:ident : $t ← $e₁ ]. $e₂) => `(Later.ap (next[]. (fun $x : $t => $e₂)) $e₁)
+  | `(term| next[ $x:ident ← $e₁, $es,* ]. $e₂) => `(Later.ap (next[ $es,* ]. (fun $x => $e₂)) $e₁)
+  | `(term| next[ $x:ident : $t ← $e₁, $es,* ]. $e₂) => `(Later.ap (next[ $es,* ]. (fun $x : $t => $e₂)) $e₁)
 
 axiom Later.eq {α : Sort u} {a b : α} : ▹ (a = b) ↔ (next[].a) = (next[].b)
 axiom Later.ap.compute {α β : Sort u} (f : α → β) (a : α) : Later.ap (next[].f) (next[].a) = next[].(f a)
-axiom Later.ap.assoc {α β : Sort u} (f : α → β) (a : α) : Later.ap (next[].f) (next[].a) = next[].(f a)
+axiom Later.ap.assoc1 {α β : Sort u} (f : α → β) (a : α) : Later.ap (next[].f) (next[].a) = next[].(f a)
+axiom Later.ap.assoc2 {α β γ : Sort u} (f : α → β) (g : β → γ) (la : ▹ α) : Later.ap (next[].g) (Later.ap (next[].f) la) = Later.ap (next[]. fun a => g (f a)) la
 axiom Later.ap.id {α β : Sort u} (f : α → β) (a : ▹ α) : Later.ap (next[].id) a = a
 
 axiom DLater : ▹ (Sort u) → Sort u
@@ -55,5 +56,4 @@ def flippp {α β : Type u} : (α → Laterrr β) → Laterrr (α → β) :=
 
 @[extern "flippp"]
 axiom Later.unsafeFlip {α β : Type u} : (α → Later β) → Later (α → β)
-
--- axiom Later.unsafeFlip_eq {α β γ : Type u} (f : α → Later β) (h : (α → β) → γ) : (next[g ← Later.unsafeFlip f]. h g) = h <$> f a -- I'm reasonably certain that this rule is safe
+axiom Later.unsafeFlip_eq {α β : Type u} (f : α → Later β) (μ : α) : Later.ap (Later.next (fun () g => g μ)) (Later.unsafeFlip f) = f μ -- I'm reasonably certain that this rule is safe
